proof: starting tape content handling
and a nicer way to handle the interface between the num world of lists
and the int world of TMs

proofs/tm.ml
@@ -1,25 +1,20 @@
-(* bare minimum "generic" TM theory to allow proving existentials *)
+(* preliminaries - function theory *)
 
 let ITERF_DEF = define`ITERF 0 f (x:A) = x /\ ITERF (SUC n) f x = f (ITERF n f x)`;;
 let ITERF_ADD = prove(`!m n f (x:A). ITERF (m + n) f x = ITERF m f (ITERF n f x)`,
   INDUCT_TAC THEN ASM_REWRITE_TAC[ADD_CLAUSES;ITERF_DEF]);;
 
-let gtm_valid_DEF = define`gtm_valid (tt:num->bool->num#bool#bool) st <=> ~(st = 0) /\ !b. FST(tt 0 b) = 0 /\ !i. i <= st ==> FST (tt i b) <= st` ;;
-let tape_shift_DEF = define`shift i (tp:int->bool) = \j. tp (i+j)`;;
-let tape_write_DEF = define`write v (tp:int->bool) = \i. if i = &0 then v else tp i`;;
-let halted_DEF = define`halted = 0,\(i:int).F`;;
-let gtm_step_DEF = define`gtm_step tt (st:num,t) = let ns,m,w = tt st (t (&0)) in if ns=0 then halted else ns,shift (if m then &1 else -- &1) (write w t)` ;;
+(* preliminaries - fast maps
 
-let nqlroot = Sys.getenv "NQLROOT";;
-let tm_lines = In_channel.with_open_text (nqlroot ^ "/machines/2017-zf-sorear-748/zf2.tm") In_channel.input_lines ;;
-let tm_states_tok = List.map (String.split_on_char ' ') ("HALT = 0 L HALT 0 L HALT" :: tm_lines) ;;
-let state_of_name n = Option.get (List.find_index (fun tp -> n = (List.hd tp)) tm_states_tok) ;;
-let name_of_state s = List.hd (List.nth tm_states_tok s) ;;
-let next_info toks i = state_of_name (List.nth toks i) ;;
-let toks_to_state_info [name;_;w0;m0;ns0;w1;m1;ns1] = (name,(state_of_name ns0,m0="R",w0="1"),(state_of_name ns1,m1="R",w1="1")) ;;
-let state_info = List.map toks_to_state_info tm_states_tok ;;
+   hol-light's built in definition by cases is far, far too slow to handle our
+   transition table
 
-let mk_bool b = if b then `T` else `F` ;;
+   maps are typed as functions, but have a recursive representation that allows
+   logarithmic time evaluation without alpha conversion. the base concept is
+   similar to sptree from HOL4, but simplified for our use case
+   
+   imprecise = few guarantees on value outside provided alist. a precise mode
+   is possible but requires ~twice the term nodes *)
 
 let nmap_node_DEF = define`NMAP_NODE l r = \i. (if ODD i then r else l) (i DIV 2):A` ;;
 let nmap_leaf_DEF = define`NMAP_LEAF v f = \i. if i = 0 then v else f:A` ;;
@@ -37,7 +32,6 @@ let nmap_FORALL = prove(
  `((\m. !i. P (m i:A)) (NMAP_NODE x y) <=> (\m. !i. P (m i)) x /\ (\m. !i. P (m i)) y) /\ ((\m. !i. P (m i)) (NMAP_LEAF a b) <=> P a /\ P b)`,
   (CONJ_TAC THEN EQ_TAC THEN SIMP_TAC[nmap_node_DEF;nmap_leaf_DEF;COND_RAND;COND_RATOR;COND_ID] THEN REPEAT STRIP_TAC) THENL
     (List.map (fun t -> POP_ASSUM (MP_TAC o SPEC t)) [`BIT0 i`;`BIT1 i`;`0`;`1`]) THEN REWRITE_TAC[UNBIT01;ARITH_EQ]);;
-
 
 let mk_nmap_imprecise def =
   let leaf = mk_const("NMAP_LEAF",[type_of def,aty]) in
@@ -58,6 +52,43 @@ let bmap_FORALL = prove(`(\m. !b. P (m b:A)) (BMAP f t) <=> P f /\ P t`, REWRITE
 
 let mk_bmap f t = mk_binop (mk_const("BMAP",[type_of f,aty])) f t ;;
 
+(* definition of a general TM
+
+   we do everything concretely, but want to be able to present an existential
+   theorem later "there is an <X> state TM that does <Y>"
+   
+   head positions are implicit, we limit to a single tape and 2 symbols, states
+   are num indexed (to avoid type variables in the sequel), the transition
+   table takes the current state and symbol and produces the new state,
+   movement direction, and new symbol.
+   
+   being halted is considered an update and associated with state 0 for
+   totality reasons, valid TMs will not leave state 0. similarly, the initial
+   state is always 1 *)
+
+let gtm_valid_DEF = define`gtm_valid (tt:num->bool->num#bool#bool) st <=> ~(st = 0) /\ !b. FST(tt 0 b) = 0 /\ !i. i <= st ==> FST (tt i b) <= st` ;;
+let tape_shift_DEF = define`shift i (tp:int->bool) = \j. tp (i+j)`;;
+let tape_write_DEF = define`write v (tp:int->bool) = \i. if i = &0 then v else tp i`;;
+let halted_DEF = define`halted = 0,\(i:int).F`;;
+let gtm_step_DEF = define`gtm_step tt (st:num,t) = let ns,m,w = tt st (t (&0)) in if ns=0 then halted else ns,shift (if m then &1 else -- &1) (write w t)` ;;
+
+(* loading and parsing .tm files emitted by nqlaconic
+
+   state_info is a list of (name,when symbol 0,when symbol 1) with behaviors
+   represented as transition table values. name_to_state is also important and
+   will drive most proving *)
+
+let nqlroot = Sys.getenv "NQLROOT";;
+let tm_lines = In_channel.with_open_text (nqlroot ^ "/machines/2017-zf-sorear-748/zf2.tm") In_channel.input_lines ;;
+let tm_states_tok = List.map (String.split_on_char ' ') ("HALT = 0 L HALT 0 L HALT" :: tm_lines) ;;
+let state_of_name n = Option.get (List.find_index (fun tp -> n = (List.hd tp)) tm_states_tok) ;;
+let name_of_state s = List.hd (List.nth tm_states_tok s) ;;
+let next_info toks i = state_of_name (List.nth toks i) ;;
+let toks_to_state_info [name;_;w0;m0;ns0;w1;m1;ns1] = (name,(state_of_name ns0,m0="R",w0="1"),(state_of_name ns1,m1="R",w1="1")) ;;
+let state_info = List.map toks_to_state_info tm_states_tok ;;
+
+let mk_bool b = if b then `T` else `F` ;;
+
 (* subst a large term into the body of an abs is slow since it needs to be checked for bound variables; possibly exponential nested alpha, def linear *)
 (* comparing rigorously identical terms is fast *)
 (* assumption lists are linear *)
@@ -68,17 +99,7 @@ let mk_bmap f t = mk_binop (mk_const("BMAP",[type_of f,aty])) f t ;;
 (* top_depth: exhaust, recurse, alternate trying root once and recursing *)
 (* top_sweep: exhaust then recurse *)
 
-
-(* too slow - 20+ min
-
-let triple_def (s,b) (ns,m,w) = mk_eq(mk_binop(mk_var("transition_map",`num -> bool -> num#bool#bool`), mk_small_numeral s, mk_bool b), mk_pair(mk_small_numeral ns, mk_pair(mk_bool m, mk_bool w))) in
-list_mk_conj (List.concat_map (fun (_,t0,t1) -> [triple_def t0; triple_def t1]))a
-
-let transition_map_DEF =
-  let triple_def (s,b) (ns,m,w) = mk_eq(mk_binop (mk_var("transition_map",`:num -> bool -> num#bool#bool`)) (mk_small_numeral s) (mk_bool b), mk_pair(mk_small_numeral ns, mk_pair(mk_bool m, mk_bool w))) in
-  state_info |> List.mapi (fun i (_,t0,t1) -> [triple_def (i,false) t0; triple_def (i,true) t1]) |> List.concat |> list_mk_conj |> define;;
-
-*)
+(* construct and prove validity of loaded transition table *)
 
 let transition_table_DEF =
   let triple (ns,m,w) = mk_pair(mk_small_numeral ns, mk_pair(mk_bool m, mk_bool w)) in
@@ -89,3 +110,47 @@ let transition_table_LIMIT = CONV_RULE (SIMP_CONV[]) ((PURE_REWRITE_CONV [transi
   `(\m. !i. (\n. !b. FST (n b) <= 748) (m i)) transition_table`);;
 
 let transition_table_VALID = prove(`gtm_valid transition_table 748`, REWRITE_TAC[gtm_valid_DEF;transition_table_LIMIT;FORALL_BOOL_THM;transition_table_DEF;nmap_CLAUSES;bmap_CLAUSES;ARITH_EQ]);;
+
+    (* to convert ground terms, may become optimized *)
+let transition_table_CONV = REWRITE_CONV[transition_table_DEF;nmap_CLAUSES;bmap_CLAUSES];;
+
+(* tape handling
+
+   for the register and dispatch logic, we represent the tape at the bit level,
+   since updates do not pass through intermediate states that are meaningful at
+   higher levels. we also support "cruft" in ignored portions of the tape,
+   because ajwade's machines use an unclean initialization process.
+
+   the initialization process itself does not have to be modeled since it
+   halts, but we need a calculation-friendly tape representation *)
+
+let list_tape_DEF = define `list_tape l tp = \i. &0 <= tp+i /\ tp+i < &(LENGTH l) /\ EL (num_of_int (tp+i)) l`;;
+let bilist_tape_DEF = define `bilist_tape ll sy rl = \i. if i = &0 then sy else let l = if i < &0 then ll else rl in let ii = num_of_int (abs i - 1) in ii < LENGTH l /\ EL ii l`;;
+
+let list_tape_SHIFT = prove(`shift j (list_tape l tp) = list_tape l (tp+j)`, SIMP_TAC[tape_shift_DEF;list_tape_DEF;INT_ADD_ASSOC]);;
+
+let NUM_OF_INT_2 = prove(`&0 <= x ==> ?z. x:int = &z`, REWRITE_TAC[EXISTS_THM;NUM_OF_INT;num_of_int] THEN MESON_TAC[]);;
+
+let list_tape_RAPPEND = prove(
+ `list_tape (APPEND l [F]) tp = list_tape l tp`,
+  REWRITE_TAC[list_tape_DEF] THEN ABS_TAC THEN ASM_CASES_TAC `&0 <= tp+i` THEN ASM_SIMP_TAC[] THEN
+  POP_ASSUM (DESTRUCT_TAC "@j. eq" o MATCH_MP NUM_OF_INT_2) THEN POP_ASSUM SUBST1_TAC THEN
+  EQ_TAC THEN SIMP_TAC[NUM_OF_INT_OF_NUM;INT_OF_NUM_LT;LENGTH_APPEND;LENGTH;EL_APPEND;ADD_CLAUSES;LT] THEN
+  INTRO_TAC "(lt|eq) el" THEN USE_THEN "el" (UNDISCH_TAC o concl) THEN ASM_SIMP_TAC[SUB_REFL;LT_REFL;EL;HD]);;
+
+let list_tape_LAPPEND = prove(
+ `list_tape (APPEND [F] l) (tp + &1) = list_tape l tp`,
+   SIMP_TAC[list_tape_DEF;APPEND;LENGTH;EL_CONS;INT_ADD_AC] THEN ABS_TAC THEN ASM_CASES_TAC `i + tp + &1 = &0` THENL[
+     MP_TAC(SPEC `&0` NUM_OF_INT) THEN ASM_SIMP_TAC[INT_LE_REFL;INT_OF_NUM_EQ] THEN ASM_ARITH_TAC;
+     ASM_REWRITE_TAC[INT_LE_LT;INT_ADD_ASSOC;GSYM INT_LE_DISCRETE;ADD1;GSYM INT_OF_NUM_ADD;INT_LT_RADD] THEN
+     REWRITE_TAC[GSYM INT_ADD_ASSOC;GSYM INT_LE_LT] THEN
+     SIMP_TAC[TAUT `(p/\q)=(p/\r)<=>(p==>q=r)`;NUM_OF_INT;INT_ADD_ASSOC] THEN FIRST_X_ASSUM (DESTRUCT_TAC "nz") THEN
+     INTRO_TAC "num" THEN USE_THEN "nz" (UNDISCH_TAC o concl) THEN REWRITE_TAC[INT_ADD_ASSOC] THEN
+     USE_THEN "num" (SUBST1_TAC o SYM) THEN REWRITE_TAC[INT_OF_NUM_CLAUSES] THEN
+     REWRITE_TAC[NUM_OF_INT_OF_NUM;GSYM ADD1;NOT_SUC] THEN REWRITE_TAC[ADD1;ADD_SUB]]);;
+
+
+
+
+let bilist_tape_READ = prove(`bilist_tape ll sy rl (&0) = sy`, REWRITE_TAC[bilist_tape_DEF]);;
+let bilist_tape_WRITE = prove(`write sy' (bilist_tape_2 ll sy rl) = (bilist_tape_2 ll sy' rl)`, SIMP_TAC[bilist_tape_DEF;tape_write_DEF]);;
